\documentclass{article}
\usepackage{amsmath}
\usepackage{amssymb}
\usepackage{amsthm}
\usepackage{graphicx}
\usepackage[margin=1.0in]{geometry}
\usepackage{fancyhdr} % for headers and footers
\usepackage{euler} % font
\usepackage[nobreak=false]{mdframed}
\usepackage{bm} % bold math for vectors
\usepackage[dvipsnames]{xcolor}
\usepackage{multicol}
\usepackage{caption}
\usepackage{hyperref} % Links

\newenvironment{greytext}{\color{Gray}}{\ignorespacesafterend}

\newcommand{\volume}{\mathop{\ooalign{\hfil$V$\hfil\cr\kern0.08em--\hfil\cr}}\nolimits} % Fluid dynamics volume

\hypersetup{
        colorlinks=true,
        linkcolor=blue,
        filecolor=magenta,      
        urlcolor=cyan,
}

\title{Axle Damping Calculation}

\author{Valmik Prabhu}

\graphicspath{ {Images/} }

\begin{document}

\maketitle

\parindent = 0pt

\subsection{Laplacian}

We start with the differential equation:
\begin{equation*}
    u(t) = m\ddot{x} + c\dot{x} + kx
\end{equation*}

We then take the Laplacian by breaking it down:
\begin{equation*}
    \mathcal{L}\{m\ddot{x} + c\dot{x} + kx\} = \mathcal{L}\{m\ddot{x}\} + \mathcal{L}\{c \dot{x}\} + \mathcal{L}\{kx\} = \mathcal{L}\{u\}
\end{equation*}

We have
\begin{gather*}
    \mathcal{L}\{m\ddot{x}\} = m(s^2 X(s) - sx(0) - \dot{x}(0)) \\
    \mathcal{L}\{c \dot{x}\} = c(sX(s) + x(0)) \\
    \mathcal{L}\{kx\} = kX(s) \\
    \mathcal{L}\{u\} = U(s)
\end{gather*}

Combining yields:
\begin{equation*}
    U(s) = m(s^2 X(s) - sx(0) - \dot{x}(0)) + c(sX(s) + x(0)) + kX(s)
\end{equation*}

To solve for $X$ it's easiest if we have $U$, which we know is a step response of unknown magnitude, and therefore is

\begin{equation*}
    U(s) = \mu \frac{1}{s}
\end{equation*}

where $\mu$ is the magnitude. Solving the equation yields: 

\begin{equation*}
    X(s) = \frac{\mu + ms\dot{x}(0) + (ms^2 + ks)x(0)}{ms^3 + cs^2 + ks}
\end{equation*}


\subsection{Inverse Laplacian}
Now we use the inverse laplacian to solve for the step response in the time domain. First we break it up:

\begin{align*}
    X(s) = & \\
    & \frac{\mu}{ms^3 + cs^2 + ks} \\
    & \frac{ms \dot{x}(0)}{ms^3 + cs^2 + ks} = \frac{m \dot{x}(0)}{ms^2 + cs + k} \\
    & \frac{(ms^2 + ks)x(0)}{ms^3 + cs^2 + ks} = \frac{(ms + k)x(0)}{ms^2 + cs + k}
\end{align*}


\subsubsection{First Part}
For the first part, it most-closely resembles this transform:
\begin{equation*}
    K\frac{a^2 + b^2}{s[(s+a^2) + b^2]} = K - Ke^{-at}(\cos(bt) + \frac{a}{b}\sin(bt))
\end{equation*}

Setting
\begin{equation*}
    K\frac{a^2 + b^2}{s[(s+a)^2 + b^2]} = \frac{\mu}{s[ms^2 + cs + k]}
\end{equation*}

We find that 
\begin{gather*}
    a = \frac{c}{2m} \\
    a^2 + b^2 = \frac{k}{m} \\
    b = \sqrt{\frac{k}{m} - \frac{c^2}{4m^2}} \\
    K = \frac{\mu}{k}
\end{gather*}

Solving back yields:

\begin{equation*}
    K\frac{a^2 + b^2}{s[(s+a)^2 + b^2]} = \frac{\frac{\mu}{k} \frac{k}{m}}{s[s^2 + \frac{c}{m}s + \frac{c^2}{4m^2} + \frac{k}{m} - \frac{c^2}{4m^2}]} = \frac{\frac{\mu}{m}}{s[s^2 + \frac{c}{m}s + \frac{k}{m}]} = \frac{\mu}{s[ms^2 + cs + k]}
\end{equation*}

So in the time domain, it's 
\begin{equation*}
    \frac{\mu}{k} - \frac{\mu}{k}e^{-\frac{c}{2m}t}(\cos(\sqrt{\frac{k}{m} - \frac{c^2}{4m^2}}t) + \frac{\frac{c}{2m}}{\sqrt{\frac{k}{m} - \frac{c^2}{4m^2}}}\sin(\sqrt{\frac{k}{m} - \frac{c^2}{4m^2}}t))
\end{equation*}

\subsubsection{Second Part}
The second resembles
\begin{equation*}
    K\frac{b}{(s+a)^2 + b^2} = Ke^{-at}\sin(bt)
\end{equation*}

Setting
\begin{equation*}
    K\frac{b}{(s+a)^2 + b^2} = \frac{m \dot{x}(0)}{ms^2 + cs + k}
\end{equation*}

We find that
\begin{gather*}
    a = \frac{c}{2m} \\
    a^2 + b^2 = \frac{k}{m} \\
    b = \sqrt{\frac{k}{m} - \frac{c^2}{4m^2}} \\
    K = \frac{\dot{x}(0)}{\sqrt{\frac{k}{m} - \frac{c^2}{4m^2}}}
\end{gather*}

Solving back yields:
\begin{equation*}
    K\frac{b}{(s+a)^2 + b^2} = \frac{\frac{\dot{x}(0)}{\sqrt{\frac{k}{m} - \frac{c^2}{4m^2}}} \sqrt{\frac{k}{m} - \frac{c^2}{4m^2}}}{s^2 + \frac{c}{m} + \frac{c^2}{4m^2} + \frac{k}{m} - \frac{c^2}{4m^2}} = \frac{\dot{x}(0)}{s^2 + \frac{c}{m}s + \frac{k}{m}} = \frac{m\dot{x}(0)}{ms^2 + cs + k}
\end{equation*}

So in the time domain, it's
\begin{equation*}
    \frac{\dot{x}(0)}{\sqrt{\frac{k}{m} - \frac{c^2}{4m^2}}} e^{-\frac{c}{2m}t}\sin(\sqrt{\frac{k}{m} - \frac{c^2}{4m^2}}t)
\end{equation*}


\subsubsection{Third Part}
The third resembles:
\begin{equation*}
    K\frac{s + a}{(s+a)^2 + b^2} = Ke^-{at}cos(bt)
\end{equation*}

Setting
\begin{equation*}
    K\frac{s + a}{(s+a)^2 + b^2} = \frac{(ms + k)x(0)}{ms^2 + cs + k}
\end{equation*}

We find that
\begin{gather*}
    a = \frac{c}{2m} \\
    a^2 + b^2 = \frac{k}{m} \\
    b = \sqrt{\frac{k}{m} - \frac{c^2}{4m^2}} \\
    K = ????
\end{gather*}

Just realized, we don't actually need to know the forms of the constants, we just need to know that they exist.

\subsection{Putting it together}

Solving for the first two terms gives us this equation

We have this equation:
\begin{equation*}
    \frac{\mu}{k} - \frac{\mu}{k}e^{-\frac{c}{2m}t}(\cos(\sqrt{\frac{k}{m} - \frac{c^2}{4m^2}}t) + \frac{\frac{c}{2m}}{\sqrt{\frac{k}{m} - \frac{c^2}{4m^2}}}\sin(\sqrt{\frac{k}{m} - \frac{c^2}{4m^2}}t)) + \frac{\dot{x}(0)}{\sqrt{\frac{k}{m} - \frac{c^2}{4m^2}}} e^{-\frac{c}{2m}t}\sin(\sqrt{\frac{k}{m} - \frac{c^2}{4m^2}}t)
\end{equation*}

But this is hard to fit to, so we'll use:
\begin{equation*}
    K_1 - K_1e^{-at}(\cos(bt) + \frac{a}{b}\sin(bt)) + K_2e^{-at}\sin(bt)
\end{equation*}

With
\begin{gather*}
    a = \frac{c}{2m} \\
    a^2 + b^2 = \frac{k}{m} \\
    b = \sqrt{\frac{k}{m} - \frac{c^2}{4m^2}} \\
    K_1 = \frac{\mu}{k} \\
    K_2 = \frac{\dot{x}(0)}{\sqrt{\frac{k}{m} - \frac{c^2}{4m^2}}}
\end{gather*}

Fitting in Matlab doesn't do well enough, so we use:

\begin{equation*}
    K_1 - K_1e^{-at}(\cos(bt) + \frac{a}{b}\sin(bt)) + K_2e^{-at}\sin(bt) + K_3 e^{-at}\cos(bt)
\end{equation*}





\end{document}